Add support for encoding lists of nums as a single num, and provide the obvious sample of functions over such lists.

src/num/extra_theories/numpairScript.sml
@@ -207,5 +207,79 @@ val nfst_le = store_thm(
   DECIDE_TAC);
 val nsnd_le = store_thm("nsnd_le", ``nsnd n ≤ n``, SRW_TAC [][nsnd_def]);
 
+(* ----------------------------------------------------------------------
+    lists of naturals encoded as naturals 
+   ---------------------------------------------------------------------- *)
+
+val _ = overload_on ("nnil", ``0``);
+val _ = overload_on ("0", ``0``);
+
+val ncons_def = Define`
+  ncons h t = h ⊗ t + 1
+`;
+
+val ncons_11 = Store_thm(
+  "ncons_11",
+  ``(ncons x y = ncons h t) ⇔ (x = h) ∧ (y = t)``,
+  SRW_TAC [][ncons_def]);
+val ncons_not_nnil = Store_thm(
+  "ncons_not_nnil",
+  ``ncons x y ≠ nnil``,
+  SRW_TAC [ARITH_ss][ncons_def]);
+
+val nlistrec_defn = Defn.Hol_defn "nlistrec" `
+  nlistrec n f l = if l = 0 then n
+                   else f (nfst (l - 1)) (nsnd (l - 1)) 
+                          (nlistrec n f (nsnd (l - 1)))
+`;
+
+val (nlistrec_def, nlistrec_ind) = Defn.tprove(
+  nlistrec_defn,
+  WF_REL_TAC `measure (SND o SND)` THEN 
+  STRIP_TAC THEN ASSUME_TAC (Q.INST [`n` |-> `l - 1`] nsnd_le) THEN 
+  DECIDE_TAC);
+
+val nlistrec_thm = Store_thm(
+  "nlistrec_thm",
+  ``(nlistrec n f nnil = n) ∧
+    (nlistrec n f (ncons h t) = f h t (nlistrec n f t))``,
+  CONJ_TAC THEN1 SRW_TAC [][Once nlistrec_def] THEN 
+  CONV_TAC (LAND_CONV (ONCE_REWRITE_CONV [nlistrec_def])) THEN 
+  SRW_TAC [ARITH_ss][ncons_def]);
+
+val nlist_ind = store_thm(
+  "nlist_ind",
+  ``∀P. P 0 ∧ (∀h t. P t ⇒ P (ncons h t)) ⇒ ∀n. P n``,
+  GEN_TAC THEN STRIP_TAC THEN
+  Q_TAC SUFF_TAC `∀(n:'a) (f:num -> num -> 'a -> 'a) l. P l` 
+    THEN1 METIS_TAC [] THEN
+  HO_MATCH_MP_TAC nlistrec_ind THEN REPEAT STRIP_TAC THEN 
+  Cases_on `l` THEN SRW_TAC [][] THEN 
+  `SUC n = ncons (nfst n) (nsnd n)` by SRW_TAC [][ncons_def, ADD1] THEN 
+  SRW_TAC [][]);
+
+val nlen_def = Define`nlen = nlistrec 0 (λn t r. r + 1)`
+
+val nlen_thm = Store_thm(
+  "nlen_thm",
+  ``(nlen nnil = 0) ∧ (nlen (ncons h t) = nlen t + 1)``,
+  SRW_TAC [][nlen_def]);
+
+val nmap_def = Define`nmap f = nlistrec 0 (λn t r. ncons (f n) r)`
+val nmap_thm = Store_thm(
+  "nmap_thm",
+  ``(nmap f nnil = nnil) ∧
+    (nmap f (ncons h t) = ncons (f h) (nmap f t))``,
+  SRW_TAC [][nmap_def]);
+
+val nfoldl_def = Define`
+  nfoldl f a l = nlistrec (λa. a) (λn t r a. r (f n a)) l a
+`;
+val nfoldl_thm = Store_thm(
+  "nfoldl_thm",
+  ``(nfoldl f a nnil = a) ∧ (nfoldl f a (ncons h t) = nfoldl f (f h a) t)``,
+  SRW_TAC [][nfoldl_def]);
+
+
 val _ = export_theory()
 
